\section{Existence of Finite Coproducts}

\subsection{Well-definedness of $\Psi$}

For $X,Y,Z \in \catf{A}$, we define $\mathrm{dst}_{X,Y,Z} \colon (X \otimes Y)
\oplus (X \otimes Z) \to X \otimes (Y \oplus Z)$ and $\mathrm{dst}'_{X,Y,Z}
\colon (X \otimes Z) \oplus (Y \otimes Z) \to (X \oplus Y) \otimes Z$ to be
canonical isomorphisms.  For $X,Y \in \catf{A}$, we denote the zero morphism $X
\longrightarrow 0 \longrightarrow Y$ in $\catf{A}$ by $O_{X,Y}$, and for
$X,Y,Z,W \in \catf{A}$, we define $\xi_{X,Y,Z,W} \colon (X \oplus Y) \otimes (Z
\oplus W) \to (X \otimes Z) \oplus (Y \otimes W)$ and $\xi'_{X,Y,Z,W} \colon (X
\otimes Z) \oplus (Y \otimes W) \to (X \oplus Y) \otimes (Z \oplus W)$ to be
unique morphisms in $\catf{A}$ such that
\begin{align*}
  \xi_{X,Y,Z} \circ (\iota_{X,Y} \otimes \iota_{Z,W}) &= \iota_{X \otimes Z,Y \otimes W}, \\
  \xi_{X,Y,Z} \circ (\iota_{X,Y} \otimes \iota'_{Z,W}) &=
  O_{X \otimes W,(X \otimes Z) \oplus (Y \otimes W)}, \\
  \xi_{X,Y,Z} \circ (\iota'_{X,Y} \otimes \iota_{Z,W}) &=
  O_{Y \otimes Z,(X \otimes Z) \oplus (Y \otimes W)}, \\
  \xi_{X,Y,Z} \circ (\iota'_{X,Y} \otimes \iota'_{Z,W}) &=
  \iota'_{X \otimes Z,Y \otimes W}, \\
  \xi'_{X,Y,Z,W} \circ \iota_{X \otimes Z,Y \otimes W} &= \iota_{X,Y} \otimes \iota_{Z,W}, \\
  \xi'_{X,Y,Z,W} \circ \iota'_{X \otimes Z,Y \otimes W} &= \iota'_{X,Y} \otimes \iota'_{Z,W}.
\end{align*}
We note that we have $\xi_{X,Y,Z,W} \circ \xi'_{X,Y,Z,W} = \Id_{(X \otimes Z)
\oplus (Y \otimes W)}$ and $\Psi_{X,Y,Z}((f,U),(g,V)) =
(\mathrm{dst}'_{Z,U,V} \circ (f \oplus g) \circ \xi_{X,Y,U,V},U \oplus V)$
for $(f,U) \colon X \to Z$ nad $(g,V) \colon Y \to Z$.

For $(f,U) \sim (f',U') \colon X \to Z$ and $(g,V) \colon Y \to Z$,
we show
\begin{equation*}
  \Psi_{X,Y,Z}((f,U),(g,V)) \sim \Psi_{X,Y,Z}((f',U'),(g,V))
\end{equation*}
by induction on the definition of $\sim$. 
When $f = h \circ (X \otimes u)$ and $f' = (Z \otimes u) \circ h$
for some $u \colon U \to U'$ and $h \colon X \otimes U' \to Z \otimes U$,
we have
\begin{align*}
  \Psi_{X,Y,Z}((f,U),(g,V)) &= (\mathrm{dst}'_{Z,U,V} \circ
  (h \oplus g) \circ \xi_{X,Y,U',V} \circ ((X \oplus Y) \otimes (u \oplus V)),U \oplus V), \\
  \Psi_{X,Y,Z}((f',U'),(g,V)) &= ((Z \otimes (u \oplus V)) \circ \mathrm{dst}'_{Z,U,V} \circ
  (h \oplus g) \circ \xi_{X,Y,U',V},U' \oplus V).
\end{align*}
Hence, $\Psi_{X,Y,Z}((f,U),(g,V)) = \Psi_{X,Y,Z}((f',U'),(g,V))$.
When $U' = U \otimes T$ and 
\begin{equation*}
  f = f_{1} \circ f_{2}, \qquad
  f' = (f_{1} \otimes T) \circ (W \otimes \sigma_{T,T}) \circ (f_{2} \otimes T)
\end{equation*}
for some $f_{1} \colon W \otimes T \to Z \otimes U$
and $f_{2} \colon X \otimes U \to W \otimes T$, we have
\begin{equation*}
  \Psi_{X,Y,Z}((f',U'),(g,V))
  = ((Z \otimes \xi'_{U,V,T,I}) \circ h \circ ((X \oplus Y) \otimes \xi_{U,V,T,I}),
  (U \oplus V) \otimes (T \oplus I))
\end{equation*}
where $g = \mathrm{dst}'_{Z,U',V} \circ (f' \oplus g) \circ \xi_{X,Y,U',V}$.
Using distributivity of coproducts, we can check
\begin{multline*}
  (Z \otimes \xi'_{U,V,T,I}) \circ h \circ ((X \oplus Y) \otimes \xi_{U,V,T,I}) = \\
  (k_{1} \otimes (T \oplus I)) \circ
  ((W \oplus (Y \otimes V)) \otimes \sigma_{T \oplus I,T \oplus I}) \circ
  (k_{2} \otimes (T \oplus I))
\end{multline*}
where $k_{1} \colon (W \oplus (Y \otimes V)) \otimes (T \oplus I) \to Z \otimes (U \oplus V)$
and $k_{2} \colon (X \oplus Y) \otimes (U \oplus V) \to (W \oplus (Y \otimes V))
\otimes (T \oplus I)$ in $\catf{A}$ are given by
\begin{align*}
  k_{1} &= \mathrm{dst}'_{Z,U,V} \circ (f_{1} \oplus g) \circ \xi_{W,Y \otimes V,T,I} \\
  k_{2} &= \xi'_{W,Y \otimes V,T,I} \circ (f_{2} \oplus (Y \otimes V)) \circ \xi_{X,Y,U,V} 
\end{align*} 
Hence, $\Psi_{X,Y,Z}((f',U'),(g,V)) = (k_{1} \circ k_{2},U \oplus V) =
\Psi_{X,Y,Z}((f,U),(g,V))$.

\subsection{Injectivity of $\Phi$}

We show that $\Psi_{X,Y,Z}(\Phi_{X,Y,Z}(f,U))$ is equal to $(f,U)$ for
any $(f,U) \colon X \oplus Y \to Z$ in $\tra{A}$. We have
\begin{equation*}
  \Psi_{X,Y,Z}(\Phi_{X,Y,Z}(f,U)) =
  (\mathrm{dst}'_{Z,U,U} \circ (f_{1} \oplus f_{2}) \circ h_{X,Y,U,U}, U \oplus U)
\end{equation*}
where
\begin{equation*}
  f_{1} = f \circ (\iota_{X,Y} \otimes U), \qquad
  f_{2} = f \circ (\iota'_{X,Y} \otimes U).
\end{equation*}
Let $g_{1} \colon (X \oplus Y) \otimes (U \oplus U) \to (X \oplus Y) \otimes U$
and $g_{2} \colon (X \oplus Y) \otimes U \to Z \otimes (U \oplus U)$ be
\begin{align*}
  g_{1} &= \mathrm{dst}_{X,Y,U} \circ h_{X,Y,U,U}, \\
  g_{2} &= \mathrm{dst}'_{Z,U,U} \circ (f_{1} \oplus f_{2}) \circ \mathrm{dst}_{X,Y,U}^{-1}
\end{align*}
Then
\begin{equation*}
  \Psi_{X,Y,Z}(\Phi_{X,Y,Z}(f,U))
  = ((g_{2} \otimes U) \circ (Z \otimes \sigma_{U,U}) \circ (g_{1} \otimes U),
  (U \oplus U) \otimes U).
\end{equation*}
Let $h_{1} \colon (X \oplus Y) \otimes U \to (X \oplus Y) \otimes (U \oplus U)$
and $h_{2} \colon (X \oplus Y) \otimes (U \oplus U) \to Z \otimes U$ be
morphisms in $\catf{A}$ given by
\begin{align*}
  h_{1} &= \xi'_{X,Y,U,U} \circ \mathrm{dst}_{X,Y,U}^{-1} \\
  h_{2} &= f \circ \mathrm{dst}_{X,Y,U} \circ \xi_{X,Y,U,U}.
\end{align*}
Because $h_{2} \circ h_{1} = f$ and
\begin{multline*}
  (Z \otimes \sigma_{U \oplus U,U}) \circ
  (g_{2} \otimes U) \circ (Z \otimes \sigma_{U,U}) \circ (g_{1} \otimes U)
  \circ ((X \oplus Y) \otimes \sigma_{U,U \oplus U})
  = \\
  (h_{2} \otimes (U \oplus U)) \circ ((Z \oplus Z) \otimes \sigma_{U \oplus U,U \oplus U})
  \circ (h_{1} \otimes (U \oplus U)),
\end{multline*}
we obtain $(f,U) = \Psi_{X,Y,Z} (\Phi_{X,Y,Z}(f,U))$.

\subsection{Surjectivity of $\Phi$}

We show that $\Phi_{X,Y,Z} (\Psi_{X,Y,Z}((f,U),(g,V)))$ is equal to
$((f,U),(g,V))$ for any pair $(f,U) \colon X \to Z$ and $(g,V) \colon
Y \to Z$. Let $h \colon (X \oplus Y) \otimes (U \oplus V) \to
Z \otimes (U \oplus V)$ be
\begin{equation*}
  \mathrm{dst}'_{Z,U,V} \circ (f \oplus g) \circ h_{X,Y,U,V}.
\end{equation*}
Then $\Phi_{X,Y,Z} (\Psi_{X,Y,Z}( (f,U), (g,V) )$ is equal to a pair
\begin{equation*}
  ((h \circ (\iota_{X,Y} \otimes (U \oplus V)),U \oplus V),
  (h \circ (\iota'_{X,Y} \otimes (U \oplus V)),U \oplus V)).
\end{equation*}
Let $p \colon U \oplus V \to U$ be a unique morphism in $\catf{A}$
such that $p \circ \iota_{U,V} = \Id_{U}$ and $p \circ \iota'_{U,V} =
O_{V,U}$. Then we have
\begin{equation*}
  (h \circ (\iota_{X,Y} \otimes (U \oplus V)),U \oplus V)
  = ((Z \otimes \iota_{U,V}) \circ f \circ (X \otimes p), U \oplus V) \\
  = (f,U).
\end{equation*}
We can similarly show that $(h \circ (\iota'_{X,Y} \otimes (U \oplus V)),U
\oplus V)$ is equal to $(g,V)$.


